data/finmap.lean
@@ -1,0 +1,173 @@
+import data.list.alist data.multiset data.pfun
+
+universes u v w
+open list
+
+namespace multiset
+variables {α : Type*} {β : α → Type*}
+
+def knodup (s : multiset (sigma β)) : Prop :=
+quot.lift_on s list.knodup (λ s t p, propext $ perm_knodup p)
+
+@[simp] theorem coe_knodup {l : list (sigma β)} : @knodup α β l ↔ l.knodup := iff.rfl
+
+end multiset
+
+structure finmap (α : Type u) (β : α → Type v) : Type (max u v) :=
+(val : multiset (sigma β))
+(nd : val.knodup)
+
+def alist.to_finmap {α β} (s : alist α β) : finmap α β := ⟨s.val, s.nd⟩
+local notation `⟦`:max a `⟧`:0 := alist.to_finmap a
+
+theorem alist.to_finmap_eq {α β} {s₁ s₂ : alist α β} :
+  ⟦s₁⟧ = ⟦s₂⟧ ↔ s₁.val ~ s₂.val :=
+by cases s₁; cases s₂; simp [alist.to_finmap]
+
+@[simp] theorem alist.to_finmap_val {α β} (s : alist α β) : ⟦s⟧.val = s.val := rfl
+
+namespace finmap
+variables {α : Type u} {β : α → Type v}
+open alist
+
+@[elab_as_eliminator] def lift_on
+  {γ} (s : finmap α β) (f : alist α β → γ)
+  (H : ∀ a b : alist α β, a.val ~ b.val → f a = f b) : γ :=
+begin
+  refine (quotient.lift_on s.1 (λ l, (⟨_, λ nd, f ⟨l, nd⟩⟩ : roption γ))
+    (λ l₁ l₂ p, roption.ext' (perm_knodup p) _) : roption γ).get _,
+  { exact λ h₁ h₂, H _ _ (by exact p) },
+  { have := s.nd, rcases s.val with ⟨l⟩, exact id }
+end
+
+@[simp] theorem lift_on_to_finmap {γ} (s : alist α β) (f : alist α β → γ) (H) :
+  lift_on ⟦s⟧ f H = f s := by cases s; refl
+
+@[elab_as_eliminator] theorem induction_on
+  {C : finmap α β → Prop} (s : finmap α β) (H : ∀ a, C ⟦a⟧) : C s :=
+by rcases s with ⟨⟨a⟩, h⟩; exact H ⟨a, h⟩
+
+@[extensionality] theorem ext : ∀ {s t : finmap α β}, s.val = t.val → s = t
+| ⟨l₁, h₁⟩ ⟨l₂, h₂⟩ H := by congr'
+
+instance : has_mem α (finmap α β) := ⟨λ a s, ∃ b : β a, sigma.mk a b ∈ s.val⟩
+
+theorem mem_def {a : α} {s : finmap α β} :
+  a ∈ s ↔ ∃ b : β a, sigma.mk a b ∈ s.val := iff.rfl
+
+@[simp] theorem mem_to_finmap {a : α} {s : alist α β} :
+  a ∈ ⟦s⟧ ↔ a ∈ s := iff.rfl
+
+def keys (s : finmap α β) : multiset α := s.val.map sigma.fst
+
+@[simp] theorem keys_to_finmap (s : alist α β) :
+  keys ⟦s⟧ = s.keys := rfl
+
+theorem mem_keys {a : α} {s : finmap α β} : a ∈ s.keys ↔ a ∈ s :=
+induction_on s $ λ s, mem_keys
+
+theorem keys_nodup (s : finmap α β) : s.keys.nodup :=
+induction_on s $ λ s, s.keys_nodup
+
+instance : has_emptyc (finmap α β) := ⟨⟨0, knodup_nil⟩⟩
+
+@[simp] theorem empty_to_finmap (s : alist α β) :
+  (⟦∅⟧ : finmap α β) = ∅ := rfl
+
+theorem not_mem_empty_val {s : sigma β} : s ∉ (∅ : finmap α β).val :=
+multiset.not_mem_zero _
+
+theorem not_mem_empty {a : α} : a ∉ (∅ : finmap α β) :=
+λ ⟨b, h⟩, not_mem_empty_val h
+
+@[simp] theorem keys_empty : (∅ : finmap α β).keys = 0 := rfl
+
+def singleton (a : α) (b : β a) : finmap α β :=
+⟨⟨a, b⟩::0, knodup_singleton _⟩
+
+@[simp] theorem keys_singleton (a : α) (b : β a) : (singleton a b).keys = [a] := rfl
+
+variables [decidable_eq α]
+
+def lookup (a : α) (s : finmap α β) : option (β a) :=
+lift_on s (lookup a) (λ s t, perm_lookup)
+
+@[simp] theorem lookup_to_finmap (a : α) (s : alist α β) :
+  lookup a ⟦s⟧ = s.lookup a := rfl
+
+theorem lookup_is_some {a : α} {s : finmap α β} :
+  (s.lookup a).is_some ↔ a ∈ s :=
+induction_on s $ λ s, alist.lookup_is_some
+
+instance (a : α) (s : finmap α β) : decidable (a ∈ s) :=
+decidable_of_iff _ lookup_is_some
+
+def insert (a : α) (b : β a) (s : finmap α β) : finmap α β :=
+lift_on s (λ t, ⟦insert a b t⟧) $
+λ s₁ s₂ p, to_finmap_eq.2 $ perm_insert p
+
+@[simp] theorem insert_to_finset (a : α) (b : β a) (s : alist α β) :
+  insert a b ⟦s⟧ = ⟦s.insert a b⟧ := by simp [insert]
+
+@[simp] theorem insert_of_pos {a : α} {b : β a} {s : finmap α β} : a ∈ s →
+  insert a b s = s :=
+induction_on s $ λ ⟨s, nd⟩ h, congr_arg to_finmap $
+insert_of_pos (mem_to_finmap.2 h)
+
+theorem insert_val_of_neg {a : α} {b : β a} {s : finmap α β} : a ∉ s →
+  (insert a b s).val = ⟨a, b⟩ :: s.val :=
+induction_on s $ λ s h,
+by simp [insert_val_of_neg (mt mem_to_finmap.1 h)]
+
+@[simp] theorem keys_insert (a : α) (b : β a) (s : finmap α β) :
+  (insert a b s).keys = s.keys.ndinsert a :=
+induction_on s $ λ s, by simp
+
+@[simp] theorem mem_insert {a a' : α} {b : β a} {s : finmap α β} :
+  a' ∈ insert a b s ↔ a' = a ∨ a' ∈ s :=
+by rw [← mem_keys, ← mem_keys]; simp
+
+def replace (a : α) (b : β a) (s : finmap α β) : finmap α β :=
+lift_on s (λ t, ⟦replace a b t⟧) $
+λ s₁ s₂ p, to_finmap_eq.2 $ perm_replace p
+
+@[simp] theorem replace_to_finset (a : α) (b : β a) (s : alist α β) :
+  replace a b ⟦s⟧ = ⟦s.replace a b⟧ := by simp [replace]
+
+@[simp] theorem keys_replace (a : α) (b : β a) (s : finmap α β) :
+  (replace a b s).keys = s.keys :=
+induction_on s $ λ s, by simp
+
+@[simp] theorem mem_replace {a a' : α} {b : β a} {s : finmap α β} :
+  a' ∈ replace a b s ↔ a' ∈ s :=
+induction_on s $ λ s, by simp
+
+/-- Fold a function over the key-value pairs in the map -/
+def foldl {δ : Type w} (f : δ → Π a, β a → δ)
+  (H : ∀ d a₁ b₁ a₂ b₂, f (f d a₁ b₁) a₂ b₂ = f (f d a₂ b₂) a₁ b₁)
+  (d : δ) (m : finmap α β) : δ :=
+m.val.foldl (λ d s, f d s.1 s.2) (λ d s t, H _ _ _ _ _) d
+
+def erase (a : α) (s : finmap α β) : finmap α β :=
+lift_on s (λ t, ⟦erase a t⟧) $
+λ s₁ s₂ p, to_finmap_eq.2 $ perm_erase p
+
+@[simp] theorem erase_to_finset (a : α) (s : alist α β) :
+  erase a ⟦s⟧ = ⟦s.erase a⟧ := by simp [erase]
+
+@[simp] theorem keys_erase (a : α) (s : finmap α β) :
+  (erase a s).keys = s.keys.erase a :=
+induction_on s $ λ s, by simp
+
+@[simp] theorem mem_erase {a a' : α} {s : finmap α β} : a' ∈ erase a s ↔ a' ≠ a ∧ a' ∈ s :=
+induction_on s $ λ s, by simp
+
+def extract (a : α) (s : finmap α β) : option (β a) × finmap α β :=
+lift_on s (λ t, prod.map id to_finmap (extract a t)) $
+λ s₁ s₂ p, by simp [perm_lookup p, to_finmap_eq, perm_erase p]
+
+@[simp] theorem extract_eq_lookup_erase (a : α) (s : finmap α β) :
+  extract a s = (lookup a s, erase a s) :=
+induction_on s $ λ s, by simp [extract]
+
+end finmap
