logic/basic.lean
@@ -61,6 +61,9 @@ def pempty.elim {C : Sort*} : pempty → C.
 
 instance subsingleton_pempty : subsingleton pempty := ⟨λa, a.elim⟩
 
+lemma congr_arg_heq {α} {β : α → Sort*} (f : ∀ a, β a) : ∀ {a₁ a₂ : α}, a₁ = a₂ → f a₁ == f a₂
+| a _ rfl := heq.rfl
+
 end miscellany
 
 /-
